src/hog/graph.lean
@@ -2,6 +2,7 @@
 -- graphs defined in mathlib.
 
 import .tactic
+import .tree
 
 structure simple_irreflexive_graph : Type :=
   (vertex_size : ℕ)
@@ -9,6 +10,7 @@ structure simple_irreflexive_graph : Type :=
   [edge_decidable : decidable_rel edge]
   (irreflexive : (∀ i, ¬ edge i i))
   (symmetric : (∀ i j, edge i j → edge j i))
+  (edge_size : ℕ)
 
 
 def from_edge_list (n : ℕ) (edges : list (ℕ × ℕ)) : simple_irreflexive_graph :=
@@ -17,7 +19,18 @@ def from_edge_list (n : ℕ) (edges : list (ℕ × ℕ)) : simple_irreflexive_gr
     (λ (i : fin n) (j : fin n), ¬ i = j ∧ (list.mem (i.val, j.val) edges ∨ list.mem (j.val, i.val) edges)),
   edge_decidable := begin intros i j, apply_instance end,
   irreflexive := begin intro i, tautology end,
-  symmetric := begin intros i j, tautology end
+  symmetric := begin intros i j, tautology end,
+  edge_size := edges.length
+}
+
+def from_BST (n : ℕ) (tree : BST (lex ℕ ℕ)) : simple_irreflexive_graph :=
+{ vertex_size := n,
+  edge :=
+    (λ (i : fin n) (j : fin n), ¬ i = j ∧ ((BT.edge tree.tree i.val j.val) ∨ (BT.edge tree.tree j.val i.val))),
+  edge_decidable := begin intros i j, apply_instance end,
+  irreflexive := begin intro i, tautology end,
+  symmetric := begin intros i j h, tautology end,
+  edge_size := tree.edge_size
 }
 
 @[reducible]
